src/PlutusIR.v
@@ -299,7 +299,7 @@ Inductive term :=
   | Error    : ty -> term
   | IWrap    : ty -> ty -> term -> term
   | Unwrap   : term -> term
-  | Constr   : nat -> ty -> list term -> term
+  | Constr   : ty -> nat -> list term -> term
   | Case     : ty -> term -> list term -> term
 
 with binding :=
@@ -438,7 +438,7 @@ Section term__ind.
     (H_Error   : forall t : ty, P (Error t))
     (H_IWrap   : forall (t t0 : ty) (t1 : term), P t1 -> P (IWrap t t0 t1))
     (H_Unwrap  : forall t : term, P t -> P (Unwrap t))
-    (H_Constr  : forall (i : nat) T (ts : list term), ForallP P ts -> P (Constr i T ts))
+    (H_Constr  : forall T (i : nat) (ts : list term), ForallP P ts -> P (Constr T i ts))
     (H_Case   : forall T (t : term), P t -> forall ts, ForallP P ts -> P (Case T t ts))
     .
 
@@ -476,7 +476,7 @@ Section term__ind.
       | Error ty        => H_Error ty
       | Constant c      => H_Constant c
       | Builtin f       => H_Builtin f
-      | Constr i T ts     => H_Constr i T ts (terms__ind term__ind ts)
+      | Constr T i ts     => H_Constr T i ts (terms__ind term__ind ts)
       | Case T t ts      => H_Case T t (term__ind t) ts (terms__ind term__ind ts)
     end
   with binding__ind (b : binding) : Q b :=
@@ -510,7 +510,7 @@ Section term__rect.
     (H_Error   : forall t : ty, P (Error t))
     (H_IWrap   : forall (t t0 : ty) (t1 : term), P t1 -> P (IWrap t t0 t1))
     (H_Unwrap  : forall t : term, P t -> P (Unwrap t))
-    (H_Constr  : forall (i : nat) T (ts : list term), ForallT P ts -> P (Constr i T ts))
+    (H_Constr  : forall T (i : nat) (ts : list term), ForallT P ts -> P (Constr T i ts))
     (H_Case   : forall T (t : term), P t -> forall ts, ForallT P ts -> P (Case T t ts))
     .
 
@@ -548,7 +548,7 @@ Section term__rect.
       | Error ty        => H_Error ty
       | Constant c      => H_Constant c
       | Builtin f       => H_Builtin f
-      | Constr i T ts     => H_Constr i T ts (terms__rect term__rect ts)
+      | Constr T i ts     => H_Constr T i ts (terms__rect term__rect ts)
       | Case T t ts      => H_Case T t (term__rect t) ts (terms__rect term__rect ts)
     end
   with binding__rect (b : binding) : Q b :=
@@ -581,7 +581,7 @@ Section term_rect.
     (H_Error   : forall t : ty, P (Error t))
     (H_IWrap   : forall (t t0 : ty) (t1 : term), P t1 -> P (IWrap t t0 t1))
     (H_Unwrap  : forall t : term, P t -> P (Unwrap t))
-    (H_Constr  : forall (i : nat) T (ts : list (term)), ForallT P ts -> P (Constr i T ts))
+    (H_Constr  : forall T  (i : nat) (ts : list (term)), ForallT P ts -> P (Constr T i ts))
     (H_Case   : forall T t, P t -> forall ts, ForallT P ts -> P (Case T t ts)).
 
   Context
@@ -620,7 +620,7 @@ Section term_rect.
       | Error ty        => @H_Error ty
       | Constant c      => @H_Constant c
       | Builtin f       => @H_Builtin f
-      | Constr i T ts     => @H_Constr i T ts (terms_rect' term_rect' ts)
+      | Constr T i ts     => @H_Constr T i ts (terms_rect' term_rect' ts)
       | Case T t ts      => @H_Case T t (term_rect' t) ts (terms_rect' term_rect' ts)
     end
   with binding_rect' (b : binding) : Q b :=
