src/PlutusIR/Semantics/Dynamic/AnnotationSubstitution.v
@@ -88,8 +88,8 @@ Fixpoint substA (X : string) (U : ty) (t : term) {struct t} : term :=
       IWrap (substituteT X U F) (substituteT X U T) (substA X U t0)
   | Unwrap t0 =>
       Unwrap (substA X U t0)
-  | Constr i T ts =>
-      Constr i (substituteT X U T) (map (substA X U) ts)
+  | Constr T i ts =>
+      Constr (substituteT X U T) i (map (substA X U) ts)
   | Case T t ts =>
       Case (substituteT X U T) (substA X U t) (map (substA X U) ts)
   end
